experiments/letdo_dm/AssertTest.fst
@@ -1,0 +1,110 @@
+module AssertTest
+
+open FStar.Tactics.V2
+open FStar.Monotonic.Pure
+
+open Assert
+
+(**** Test Refinements **)
+
+val incr5 (x:int{x > 5}) : r:int{r-x == 5}
+let incr5 x = x + 5
+
+val dm_incr5 (x:int{x > 5}) : dm (r:int{r-x == 5}) (requires True) (ensures fun _ -> True)
+let dm_incr5 x = do begin
+  return (incr5 x)
+end
+
+val dm_incr5' (x:int) : dm (r:int{r-x == 5}) (requires x > 5) (ensures fun _ -> True)
+let dm_incr5' x = do begin
+  let! x' = dm_refine x (fun x -> x > 5) in
+  let! r = dm_erase_refinement (fun r -> r-x'==5) (incr5 x') in
+  dm_refine r (fun r -> r-x == 5)
+end
+
+val dm_incr5'' (x:int{x > 5}) : dm int (requires True) (ensures fun r -> r-x == 5)
+let dm_incr5'' x = do begin
+  return (incr5 x)
+end
+
+val dm_incr5''' (x:int) : dm int (requires x > 5) (ensures fun r -> r-x == 5)
+let dm_incr5''' x = do begin
+  let! y = dm_refine x (fun x -> x > 5) in
+  return #int (incr5 y) // <-- needs help here
+end
+
+val dm_incr5_dm (x:int{x > 5}) : dm (r:int{r-x == 5}) (requires True) (ensures fun _ -> True)
+let dm_incr5_dm  x = do begin
+  dm_incr5 x
+end
+
+val dm_incr5_dm' (x:int) : dm (r:int{r-x == 5}) (requires x > 5) (ensures fun _ -> True)
+let dm_incr5_dm' x = do begin
+  let! x' = dm_refine x (fun x -> x > 5) in
+  let! r = dm_erase_refinement (fun r -> r-x'==5) (incr5 x') in
+  dm_refine r (fun r -> r-x == 5)
+end
+
+val dm_incr5_dm'' (x:int{x > 5}) : dm int (requires True) (ensures fun r -> r-x == 5)
+let dm_incr5_dm'' x = do begin
+  let! y = dm_incr5 x in
+  dm_erase_refinement (fun r -> r-x == 5) y
+end
+
+val dm_incr5_dm''' (x:int) : dm int (requires x > 5) (ensures fun r -> r-x == 5)
+let dm_incr5_dm''' x = do begin
+  let! x' = dm_refine x (fun x -> x > 5) in
+  return #int (incr5 x') // <-- needs help to erase the refinement
+end
+
+(** *** Test Squash **)
+assume val p : prop
+assume val p' : prop
+assume val pure_lemma (_ : unit) : dm p (requires True) (ensures fun _ -> True)
+assume val some_f (_ : squash p) : dm unit (requires True) (ensures fun _ -> True)
+assume val some_f' : unit -> dm unit (requires p) (ensures fun _ -> p')
+
+let pure_lemma_test () : dm unit (requires True) (ensures fun _ -> True) = do begin
+  pure_lemma () ;!
+  some_f ()
+end
+
+let pure_lemma_test2 () : dm unit (requires True) (ensures fun _ -> True) = do begin
+  pure_lemma () ;!
+  some_f () ;!
+  some_f' () ;!
+  dm_assert p'
+end
+
+(** *** Test partiality **)
+// A test to make sure exfalso isn't used
+let test_assume' #a #pre (f : unit -> dm a (requires pre) (ensures fun _ -> True)) : dm a True (fun _ -> True) = do begin
+  dm_assume pre ;!
+  f ()
+end
+
+let test_assert p : dm unit (requires p) (ensures fun _ -> True) = do begin
+  dm_assert p
+end
+
+[@expect_failure]
+let partial_match (l : list int) : dm unit (requires True) (ensures fun _ -> True) = do begin
+  match l with
+  | Cons _ _ -> return ()
+  | _ -> dm_contradiction ()
+end
+
+let partial_match (l : list int) : dm unit (requires Cons? l) (ensures fun _ -> True) =
+  match l with
+  | Cons _ _ -> do begin return () end
+  | _ -> do begin dm_contradiction #unit () end
+
+[@expect_failure](** how to make this work? *)
+let partial_match (l : list int) : dm unit (requires Cons? l) (ensures fun _ -> True) =
+  match l with
+  | Cons _ _ -> do begin return () end
+
+let partial_match_pre (l : list int) : dm int (requires Cons? l) (ensures fun r -> r == List.Tot.hd l) =
+  match l with
+  | x :: r -> do begin return x end
+  | _ -> do begin dm_contradiction () end
