experiments/letdo_dm/README.md
@@ -1,23 +1,44 @@
 # Let do notation for Dijkstra Monads
 
-I'm trying to figure out if one can get rid off the F\*'s effect system.
+I'm trying to figure out if one can get rid off the F\*'s effect system
+by working directly with the monadic representation.
 
 #### Syntactic sugar
-F\*'s effect system handles many things for the user.
+F\*'s effect system handles for the user the interaction
+with squash, refinements and pattern matching (match).
+
+When working with the monadic representation directly,
+dealing with refinements and pattern matching is pretty verbose.
 This can be seen in the `Assert.fst` file, `Refinements tests`
 and `partial_match`.
+
+Also see: https://github.com/FStarLang/FStar/blob/master/examples/misc/MonadicLetBindings.fst
+
+- [ ] TODO: what else?
 
 #### Monadic Representation for the effects
 This is a problem since many of the primitive F\* effects
 do not have a monadic representation, however, they can be
-axiomatized as they are now.
-
-#### Reify/reflect
-
+axiomatized (the way they are now).
 
 #### Lifting mechanism (subeffecting)
 I have a first idea on how to approach this with type classes.
 I have something for normal monads in `TCPolyBind.fst`
 that works pretty well.
-Extending it to DMs does not seem that hard conceptually.
+Extending it to DMs does not seem conceptually complicated.
 
+#### Reify/reflect
+
+A reifiable/reflectable effect, is an effect whose computational monad
+is not hidden.
+
+To make an effect NOT reifiable,
+one can hide the computational monad behind a module interface,
+and then one has to use the subcomp combinator.
+I called it `do` since mostly one uses it only once for the entire
+body of the function. Again, when pattern matching,
+it is more complicated because one has to use it on each branch.
+This can be seen in `Assert.fsti` and `AssertTest.fst`.
+
+Would be interesting to explore if one can expose a ghost reify so that
+one is still able to reason.
